src/lib/data/Kuiper.Matrix.fsti
@@ -11,6 +11,15 @@ module SZ = FStar.SizeT
 inline_for_extraction noextract
 val gpu_matrix (et:Type0) (#rows #cols : nat) (l : mlayout rows cols) : Type0
 
+
+inline_for_extraction noextract
+val from_array
+  (#a : Type0)
+  (#rows #cols : erased nat)
+  (l : mlayout rows cols)
+  (arr : gpu_array a (mlayout_size l))
+  : gpu_matrix a l
+
 inline_for_extraction noextract
 val core
   (#et : Type)
@@ -19,13 +28,21 @@ val core
   (g : gpu_matrix et l)
   : gpu_array et (rows * cols)
 
-val core_match
+val lem_core_from_array
   (#et : Type)
   (#rows #cols : erased nat)
   (#l : mlayout rows cols)
-  (g1 g2 : gpu_matrix et l)
-  : Lemma (requires core g1 == core g2)
-          (ensures g1 == g2)
+  (g : gpu_matrix et l)
+  : Lemma (ensures from_array l (core g) == g)
+          [SMTPat (core g)]
+
+val lem_from_array_core
+  (#et : Type)
+  (#rows #cols : erased nat)
+  (#l : mlayout rows cols)
+  (p : gpu_array et (mlayout_size l))
+  : Lemma (ensures core (from_array l p) == p)
+          [SMTPat (from_array l p)]
 
 val gpu_matrix_pts_to
   (#et:Type) (#rows #cols : nat) (#l : mlayout rows cols)
@@ -66,19 +83,29 @@ fn gpu_matrix_concr
   ensures
     core g |-> to_seq l em
 
-inline_for_extraction noextract
+ghost
 fn gpu_matrix_abs
   (#et:Type)
   (#rows #cols : erased nat) (l : mlayout rows cols)
   (p : gpu_array et (mlayout_size l))
+  (#f : perm)
   (#em : ematrix et rows cols)
   requires
-    p |-> to_seq l em
-  returns
-    g' : gpu_matrix et l
+    gpu_pts_to_array p #f (to_seq l em)
   ensures
-    pure (core g' == p) **
-    (g' |-> em)
+    gpu_matrix_pts_to (from_array l p) #f em
+
+ghost
+fn gpu_matrix_abs'
+  (#et:Type)
+  (#rows #cols : erased nat) (l : mlayout rows cols)
+  (p : gpu_array et (mlayout_size l))
+  (#f : perm)
+  (#s : erased (seq et){Seq.length s == mlayout_size l})
+  requires
+    gpu_pts_to_array p #f s
+  ensures
+    gpu_matrix_pts_to (from_array l p) #f (from_seq l s)
 
 inline_for_extraction noextract
 fn gpu_matrix_alloc0
