src/lib/ghost/Kuiper.Ghost.Transpose.fst
@@ -7,7 +7,9 @@ module Repr = Kuiper.Matrix.Reprs
 open Kuiper.EMatrix
 open Kuiper.Matrix.Common
 
-inline_for_extraction noextract
+#set-options "--print_implicits"
+
+ghost
 fn ghost_transpose1
   (#et:Type)
   (#rows #cols : erased nat)
@@ -15,23 +17,19 @@ fn ghost_transpose1
   (#m : ematrix et rows cols)
   requires
     gA |-> m
-  returns
-    gA' : gpu_matrix et (Repr.col_major cols rows)
   ensures
-    pure (core gA == core gA') **
-    (gA' |-> mtranspose m)
+    row2col gA |-> mtranspose m
 {
   gpu_matrix_concr gA;
   assert (pure (Seq.equal
                   (to_seq (Repr.row_major rows cols) m)
                   (to_seq (Repr.col_major cols rows) (mtranspose m))));
-  rewrite each to_seq (Repr.row_major rows cols) m
-            as to_seq (Repr.col_major cols rows) (mtranspose m);
-  let gA' = gpu_matrix_abs (Repr.col_major cols rows) (core gA);
-  gA'
+  rewrite core gA |-> to_seq (Repr.row_major rows cols) m
+       as core gA |-> to_seq (Repr.col_major cols rows) (mtranspose m);
+  gpu_matrix_abs (Repr.col_major cols rows) (core gA);
 }
 
-inline_for_extraction noextract
+ghost
 fn ghost_transpose2
   (#et:Type)
   (#rows #cols : erased nat)
@@ -39,18 +37,52 @@ fn ghost_transpose2
   (#m : ematrix et rows cols)
   requires
     gA |-> m
-  returns
-    gA' : gpu_matrix et (Repr.row_major cols rows)
   ensures
-    pure (core gA == core gA') **
-    (gA' |-> mtranspose m)
+    col2row gA |-> mtranspose m
 {
   gpu_matrix_concr gA;
   assert (pure (Seq.equal
                   (to_seq (Repr.col_major rows cols) m)
                   (to_seq (Repr.row_major cols rows) (mtranspose m))));
-  rewrite each to_seq (Repr.col_major rows cols) m
-            as to_seq (Repr.row_major cols rows) (mtranspose m);
-  let gA' = gpu_matrix_abs (Repr.row_major cols rows) (core gA);
-  gA'
+  rewrite core gA |-> to_seq (Repr.col_major rows cols) m
+       as core gA |-> to_seq (Repr.row_major cols rows) (mtranspose m);
+  gpu_matrix_abs (Repr.row_major cols rows) (core gA);
+}
+
+ghost
+fn ghost_transpose1_back
+  (#et:Type)
+  (#rows #cols : erased nat)
+  (gA : gpu_matrix et (Repr.row_major rows cols))
+  (#m : ematrix et cols rows)
+  requires
+    row2col gA |-> m
+  ensures
+    gA |-> mtranspose m
+{
+  ghost_transpose2 (row2col gA);
+  rewrite
+    col2row (row2col gA) |-> mtranspose m
+  as
+    gA |-> mtranspose m;
+  ()
+}
+
+ghost
+fn ghost_transpose2_back
+  (#et:Type)
+  (#rows #cols : erased nat)
+  (gA : gpu_matrix et (Repr.col_major rows cols))
+  (#m : ematrix et cols rows)
+  requires
+    col2row gA |-> m
+  ensures
+    gA |-> mtranspose m
+{
+  ghost_transpose1 (col2row gA);
+  rewrite
+    row2col (col2row gA) |-> mtranspose m
+  as
+    gA |-> mtranspose m;
+  ()
 }
