scripts/debug.sh
@@ -3,8 +3,11 @@
 # Debug an smt failure by running this script with an
 # fst/fsti file as argument
 
-F="$1"
-B="$(basename "$F")"
+# F="$1"
+# B="$(basename "$F")"
 
-export O="$O --debug SMTFail --split_queries always"
-make -f verify.mk obj/$B.checked
+# export O="$O --debug SMTFail --split_queries always"
+# make -f verify.mk obj/$B.checked "$@"
+
+make prepare -j$(nproc)
+./fstar.sh --debug SMTFail --split_queries always "$@"
